src/Parser/coq_pretty_printer.ml
@@ -4,11 +4,26 @@ open Ssa_lib
 open Llvm
 
 (** Coq Pretty Printer *)
+let getRealName (id:LLVMsyntax.id) =
+	  if String.length id <= 1
+	  then id
+	  else 
+	  	if String.get id 0 = '@' or String.get id 0 = '%'
+  		then String.sub id 1 (String.length id-1)
+  		else id
+
+let rec string_of_floating_point fp =
+	match fp with
+	| LLVMsyntax.Coq_fp_float -> "float" 
+  | LLVMsyntax.Coq_fp_double -> "double" 
+  | LLVMsyntax.Coq_fp_fp128 -> "fp128" 
+  | LLVMsyntax.Coq_fp_x86_fp80 -> "x86_fp80" 
+  | LLVMsyntax.Coq_fp_ppc_fp128 -> "ppc_fp128"
+
 let rec string_of_typ ty =
   match ty with
   | LLVMsyntax.Coq_typ_int sz -> "i"^(string_of_int sz)
-	| LLVMsyntax.Coq_typ_float -> "float"
-	| LLVMsyntax.Coq_typ_double -> "double"
+	| LLVMsyntax.Coq_typ_floatpoint fp -> string_of_floating_point fp
 	| LLVMsyntax.Coq_typ_void -> "void"
 	| LLVMsyntax.Coq_typ_label -> "label"
 	| LLVMsyntax.Coq_typ_metadata -> "metadata"
@@ -25,6 +40,83 @@ and string_of_list_typ ts =
   | LLVMsyntax.Cons_list_typ (t, ts') ->  (string_of_typ t)^" "^(string_of_list_typ ts')
 	| LLVMsyntax.Nil_list_typ -> ""
 
+let string_of_bop bop =
+	match bop with
+	| LLVMsyntax.Coq_bop_add -> "add" 			
+	| LLVMsyntax.Coq_bop_sub -> "sub"
+	| LLVMsyntax.Coq_bop_mul -> "mul"
+	| LLVMsyntax.Coq_bop_udiv -> "udiv"
+	| LLVMsyntax.Coq_bop_sdiv -> "sdiv"
+	| LLVMsyntax.Coq_bop_urem -> "urem"
+	| LLVMsyntax.Coq_bop_srem -> "srem"
+	| LLVMsyntax.Coq_bop_shl -> "shl"
+	| LLVMsyntax.Coq_bop_lshr -> "lshr" 			
+	| LLVMsyntax.Coq_bop_ashr -> "ashr"
+	| LLVMsyntax.Coq_bop_and -> "and"
+	| LLVMsyntax.Coq_bop_or -> "or" 			
+	| LLVMsyntax.Coq_bop_xor -> "xor"	
+									
+let string_of_fbop fbop =
+	match fbop with
+	| LLVMsyntax.Coq_fbop_fadd -> "fadd" 			
+	| LLVMsyntax.Coq_fbop_fsub -> "fsub"
+	| LLVMsyntax.Coq_fbop_fmul -> "fmul"
+	| LLVMsyntax.Coq_fbop_fdiv -> "fdiv"
+	| LLVMsyntax.Coq_fbop_frem -> "frem"
+
+let string_of_cond cond =
+	match cond with
+	| LLVMsyntax.Coq_cond_eq -> "eq" 			
+	| LLVMsyntax.Coq_cond_ne -> "ne" 			
+	| LLVMsyntax.Coq_cond_ugt -> "ugt" 			
+	| LLVMsyntax.Coq_cond_uge -> "uge" 			
+	| LLVMsyntax.Coq_cond_ult -> "ult" 			
+	| LLVMsyntax.Coq_cond_ule -> "ule" 			
+	| LLVMsyntax.Coq_cond_sgt -> "sgt" 			
+	| LLVMsyntax.Coq_cond_sge -> "sge" 			
+	| LLVMsyntax.Coq_cond_slt -> "slt" 			
+	| LLVMsyntax.Coq_cond_sle -> "sle" 			
+
+let string_of_fcond fcond =
+	match fcond with
+	| LLVMsyntax.Coq_fcond_false -> "false" 			
+	| LLVMsyntax.Coq_fcond_oeq -> "oeq"
+	| LLVMsyntax.Coq_fcond_ogt -> "ogt" 			
+	| LLVMsyntax.Coq_fcond_oge -> "oge" 			
+	| LLVMsyntax.Coq_fcond_olt -> "olt" 			
+	| LLVMsyntax.Coq_fcond_ole -> "ole" 			
+	| LLVMsyntax.Coq_fcond_one -> "one" 			
+	| LLVMsyntax.Coq_fcond_ord -> "ord" 			
+	| LLVMsyntax.Coq_fcond_ueq -> "ueq" 			
+	| LLVMsyntax.Coq_fcond_ugt -> "ugt" 			
+	| LLVMsyntax.Coq_fcond_uge -> "uge" 			
+  | LLVMsyntax.Coq_fcond_ult -> "ult" 			
+	| LLVMsyntax.Coq_fcond_ule -> "ule" 			
+	| LLVMsyntax.Coq_fcond_une -> "une"
+  | LLVMsyntax.Coq_fcond_uno -> "uno" 			
+	| LLVMsyntax.Coq_fcond_true -> "true" 			
+	
+let string_of_extop extop =
+	match extop with
+	| LLVMsyntax.Coq_extop_s -> "sext" 			
+	| LLVMsyntax.Coq_extop_z -> "zext"
+	| LLVMsyntax.Coq_extop_fp -> "fpext"
+
+let string_of_castop castop =
+	match castop with
+	| LLVMsyntax.Coq_castop_fptoui -> "fptoui" 			
+	| LLVMsyntax.Coq_castop_fptosi -> "fptosi"	 
+	| LLVMsyntax.Coq_castop_uitofp -> "uitofp"
+	| LLVMsyntax.Coq_castop_sitofp -> "sitofp"
+  | LLVMsyntax.Coq_castop_ptrtoint -> "ptrtoint"
+	| LLVMsyntax.Coq_castop_inttoptr -> "inttoptr"
+	| LLVMsyntax.Coq_castop_bitcast -> "bitcast"
+
+let string_of_truncop truncop =
+	match truncop with
+	| LLVMsyntax.Coq_truncop_int -> "trunc" 			
+	| LLVMsyntax.Coq_truncop_fp -> "fptrunc"
+
 let rec string_of_constant c = 
 	match c with
 	| LLVMsyntax.Coq_const_int (sz, i) -> APInt.to_string i^":"^string_of_int sz
@@ -33,6 +125,35 @@ let rec string_of_constant c =
 	| LLVMsyntax.Coq_const_arr (_, cs) -> string_of_list_constant cs
 	| LLVMsyntax.Coq_const_struct cs -> string_of_list_constant cs
   | LLVMsyntax.Coq_const_gid (_,id) -> id
+	| LLVMsyntax.Coq_const_zeroinitializer _ -> "zeroinitializer"
+	| LLVMsyntax.Coq_const_floatpoint (_, f) -> string_of_float f
+	| LLVMsyntax.Coq_const_truncop (op, c, t) -> 
+    string_of_truncop op^" ("^string_of_constant c^" to "^string_of_typ t^")" 
+	| LLVMsyntax.Coq_const_extop (op, c, t) -> 
+    string_of_extop op^" ("^string_of_constant c^" to "^string_of_typ t^")" 
+	| LLVMsyntax.Coq_const_castop (op, c, t) -> 
+    string_of_castop op^" ("^string_of_constant c^" to "^string_of_typ t^")" 
+  | LLVMsyntax.Coq_const_gep (ib, c, cs) -> 
+		(
+		match ib with
+		| true ->  "gepelementptr inbounds ("^string_of_constant c^" "^string_of_list_constant cs^")"
+		| false ->  "gepelementptr ("^string_of_constant c^" "^string_of_list_constant cs^")"
+		)
+  |	LLVMsyntax.Coq_const_select (c0, c1, c2) -> 
+		"select ("^string_of_constant c0^" "^string_of_constant c1^" "^string_of_constant c2^")"	
+  |	LLVMsyntax.Coq_const_icmp (cond, c1, c2) ->
+		"icmp "^string_of_cond cond^" ("^string_of_constant c1^" "^string_of_constant c2^")"	
+  |	LLVMsyntax.Coq_const_fcmp (cond, c1, c2) ->
+		"fcmp "^string_of_fcond cond^" ("^string_of_constant c1^" "^string_of_constant c2^")"	
+  | LLVMsyntax.Coq_const_extractvalue (c, cs) ->
+		"extractvalue ("^string_of_constant c^" "^string_of_list_constant cs^")"
+  | LLVMsyntax.Coq_const_insertvalue (c1, c2, cs) ->
+		"insertvalue ("^string_of_constant c1^" "^string_of_constant c2^" "^string_of_list_constant cs^")"
+  | LLVMsyntax.Coq_const_bop (op, c1, c2) ->	
+		string_of_bop op^" ("^string_of_constant c1^" to "^string_of_constant c2^")"	
+  | LLVMsyntax.Coq_const_fbop (op, c1, c2) ->	
+		string_of_fbop op^" ("^string_of_constant c1^" to "^string_of_constant c2^")"	
+						
 and string_of_list_constant cs =
 	match cs with
   | LLVMsyntax.Cons_list_const (c, cs') ->  (string_of_constant c)^" "^(string_of_list_constant cs')
@@ -52,41 +173,6 @@ let rec string_of_list_value vs =
 	match vs with
 	| LLVMsyntax.Nil_list_value -> ""
 	| LLVMsyntax.Cons_list_value (v, vs') -> (string_of_value v)^" "^(string_of_list_value vs')
-
-let string_of_bop bop =
-	match bop with
-	| LLVMsyntax.Coq_bop_add -> "add" 			
-	| LLVMsyntax.Coq_bop_and -> "and"
-	| LLVMsyntax.Coq_bop_or -> "or" 			
-	| LLVMsyntax.Coq_bop_lshr -> "lshr" 			
-									
-let string_of_extop extop =
-	match extop with
-	| LLVMsyntax.Coq_extop_s -> "sext" 			
-	| LLVMsyntax.Coq_extop_z -> "zext"
-
-let string_of_castop castop =
-	match castop with
-	| LLVMsyntax.Coq_castop_fptoui -> "fptoui" 			
-	| LLVMsyntax.Coq_castop_fptosi -> "fptosi"	 
-	| LLVMsyntax.Coq_castop_uitofp -> "uitofp"
-	| LLVMsyntax.Coq_castop_sitofp -> "sitofp"
-  | LLVMsyntax.Coq_castop_ptrtoint -> "ptrtoint"
-	| LLVMsyntax.Coq_castop_inttoptr -> "inttoptr"
-	| LLVMsyntax.Coq_castop_bitcast -> "bitcast"
-
-let string_of_cond cond =
-	match cond with
-	| LLVMsyntax.Coq_cond_eq -> "eq" 			
-	| LLVMsyntax.Coq_cond_ne -> "ne" 			
-	| LLVMsyntax.Coq_cond_ugt -> "ugt" 			
-	| LLVMsyntax.Coq_cond_uge -> "uge" 			
-	| LLVMsyntax.Coq_cond_ult -> "ult" 			
-	| LLVMsyntax.Coq_cond_ule -> "ule" 			
-	| LLVMsyntax.Coq_cond_sgt -> "sgt" 			
-	| LLVMsyntax.Coq_cond_sge -> "sge" 			
-	| LLVMsyntax.Coq_cond_slt -> "slt" 			
-	| LLVMsyntax.Coq_cond_sle -> "sle" 			
 
 let rec string_of_list_value_l vls =
 	match vls with
@@ -117,7 +203,9 @@ let travel_terminator i =
 let travel_cmd i =
 	match i with
   | LLVMsyntax.Coq_insn_bop (id, bop, sz, v1, v2) ->
-		  eprintf "  %s = bop %s i%d %s %s\n" id (string_of_bop bop) sz (string_of_value v1) (string_of_value v2)
+		  eprintf "  %s = %s i%d %s %s\n" id (string_of_bop bop) sz (string_of_value v1) (string_of_value v2)
+  | LLVMsyntax.Coq_insn_fbop (id, fbop, fp, v1, v2) ->
+		  eprintf "  %s = %s %s %s %s\n" id (string_of_fbop fbop) (string_of_floating_point fp) (string_of_value v1) (string_of_value v2)
   | LLVMsyntax.Coq_insn_extractvalue (id, t, v, cs) ->
 		  eprintf "  %s = extractvalue %s %s %s\n" id (string_of_typ t) (string_of_value v) (string_of_list_constant cs)
   | LLVMsyntax.Coq_insn_insertvalue (id, t1, v1, t2, v2, cs) ->
@@ -134,12 +222,16 @@ let travel_cmd i =
 		  eprintf "  %s = store %s %s %s %d\n" id (string_of_typ t) (string_of_value v1) (string_of_value v2) a
   | LLVMsyntax.Coq_insn_gep (id, inbounds, t, v, vs) ->
 		  eprintf "  %s = gep %s %s %s %s\n" id (string_of_bool inbounds) (string_of_typ t) (string_of_value v) (string_of_list_value vs)
+  | LLVMsyntax.Coq_insn_trunc (id, truncop, t1, v, t2) ->
+		  eprintf "  %s = %s %s %s %s\n" id (string_of_truncop truncop) (string_of_typ t1) (string_of_value v) (string_of_typ t2)
   | LLVMsyntax.Coq_insn_ext (id, extop, t1, v, t2) ->
-		  eprintf "  %s = ext %s %s %s %s\n" id (string_of_extop extop) (string_of_typ t1) (string_of_value v) (string_of_typ t2)
+		  eprintf "  %s = %s %s %s %s\n" id (string_of_extop extop) (string_of_typ t1) (string_of_value v) (string_of_typ t2)
   | LLVMsyntax.Coq_insn_cast (id, castop, t1, v, t2) ->
-		  eprintf "  %s = cast %s %s %s %s\n" id (string_of_castop castop) (string_of_typ t1) (string_of_value v) (string_of_typ t2)
+		  eprintf "  %s = %s %s %s %s\n" id (string_of_castop castop) (string_of_typ t1) (string_of_value v) (string_of_typ t2)
   | LLVMsyntax.Coq_insn_icmp (id, cond, t, v1, v2) ->
 		  eprintf "  %s = icmp %s %s %s %s\n" id (string_of_cond cond) (string_of_typ t) (string_of_value v1) (string_of_value v2)
+  | LLVMsyntax.Coq_insn_fcmp (id, fcond, fp, v1, v2) ->
+		  eprintf "  %s = fcmp %s %s %s %s\n" id (string_of_fcond fcond) (string_of_floating_point fp) (string_of_value v1) (string_of_value v2)
   | LLVMsyntax.Coq_insn_select (id, v, t, v1, v2) ->
 		  eprintf "  %s = select %s %s %s %s\n" id (string_of_value v) (string_of_typ t) (string_of_value v1) (string_of_value v2)
   | LLVMsyntax.Coq_insn_call (id, noret, tailc, t, fid, ps) ->
@@ -173,10 +265,15 @@ let travel_fdef f =
 		eprintf "define %s %s %s\n" (string_of_typ t) fid (string_of_args args); flush_all ();
 		List.iter travel_block bs
 			  	
+let string_of_gvar_spec gs =
+	match gs with
+  | LLVMsyntax.Coq_gvar_spec_global -> "global" 					
+  | LLVMsyntax.Coq_gvar_spec_constant -> "constant"
+					
 let travel_product g =
 	match g with
-	| LLVMsyntax.Coq_product_gvar (LLVMsyntax.Coq_gvar_intro (id, t, c, a)) -> 
-		eprintf "%s = global %s %s %d\n" id (string_of_typ t) (string_of_constant c) a; 
+	| LLVMsyntax.Coq_product_gvar (LLVMsyntax.Coq_gvar_intro (id, spec, t, c, a)) -> 
+		eprintf "%s = %s %s %s %d\n" id (string_of_gvar_spec spec) (string_of_typ t) (string_of_constant c) a; 
 		flush_all ()
 	| LLVMsyntax.Coq_product_fdec f -> travel_fdec f
 	| LLVMsyntax.Coq_product_fdef f -> travel_fdef f 
@@ -187,6 +284,7 @@ let travel_layout dlt =
 	| LLVMsyntax.Coq_layout_le -> eprintf "e\n"
 	| LLVMsyntax.Coq_layout_ptr (sz, a1, a2) -> eprintf "p:%d:%d:%d\n" sz a1 a2 
 	| LLVMsyntax.Coq_layout_int (sz, a1, a2) -> eprintf "i:%d:%d:%d\n" sz a1 a2	
+	| LLVMsyntax.Coq_layout_float (sz, a1, a2) -> eprintf "f:%d:%d:%d\n" sz a1 a2	
 	| LLVMsyntax.Coq_layout_aggr (sz, a1, a2) -> eprintf "a:%d:%d:%d\n" sz a1 a2
 	| LLVMsyntax.Coq_layout_stack (sz, a1, a2) -> eprintf "s:%d:%d:%d\n" sz a1 a2
 	;
