src/ssa/opsem_conv.v
@@ -689,6 +689,9 @@ Proof.
   Case "nbBop".
     apply nsop_plus_trans with (states2:=(mkState S TD Ps (mkEC F B cs tmn (updateAddAL _ lc id0 gv3) arg0 als::EC) gl Mem0, tr)::nil); 
       try solve [auto | rewrite app_nil_end; eauto].
+  Case "nbFBop".
+    apply nsop_plus_trans with (states2:=(mkState S TD Ps (mkEC F B cs tmn (updateAddAL _ lc id0 gv3) arg0 als::EC) gl Mem0, tr)::nil); 
+      try solve [auto | rewrite app_nil_end; eauto].
   Case "nbExtractValue".
     apply nsop_plus_trans with (states2:=(mkState S TD Ps (mkEC F B cs tmn (updateAddAL _ lc id0 gv') arg0 als::EC) gl Mem0, tr)::nil); 
       try solve [auto | rewrite app_nil_end; eauto].
@@ -713,6 +716,9 @@ Proof.
   Case "nbGEP".
     apply nsop_plus_trans with (states2:=(mkState S TD Ps (mkEC F B cs tmn (updateAddAL _ lc id0 mp') arg0 als::EC) gl Mem0, tr)::nil); auto.
       rewrite app_nil_end; eauto.
+  Case "nbTrunc".
+    apply nsop_plus_trans with (states2:=(mkState S TD Ps (mkEC F B cs tmn (updateAddAL _ lc id0 gv2) arg0 als::EC) gl Mem0, tr)::nil); 
+      try solve [auto | rewrite app_nil_end; eauto].
   Case "nbExt".
     apply nsop_plus_trans with (states2:=(mkState S TD Ps (mkEC F B cs tmn (updateAddAL _ lc id0 gv2) arg0 als::EC) gl Mem0, tr)::nil); 
       try solve [auto | rewrite app_nil_end; eauto].
@@ -720,6 +726,9 @@ Proof.
     apply nsop_plus_trans with (states2:=(mkState S TD Ps (mkEC F B cs tmn (updateAddAL _ lc id0 gv2) arg0 als::EC) gl Mem0, tr)::nil); 
       try solve [auto | rewrite app_nil_end; eauto].
   Case "nbIcmp".
+    apply nsop_plus_trans with (states2:=(mkState S TD Ps (mkEC F B cs tmn (updateAddAL _ lc id0 gv3) arg0 als::EC) gl Mem0, tr)::nil); 
+      try solve [auto | rewrite app_nil_end; eauto].
+  Case "nbFcmp".
     apply nsop_plus_trans with (states2:=(mkState S TD Ps (mkEC F B cs tmn (updateAddAL _ lc id0 gv3) arg0 als::EC) gl Mem0, tr)::nil); 
       try solve [auto | rewrite app_nil_end; eauto].
   Case "nbSelect".
